Desynchronization.v
@@ -1,0 +1,272 @@
+Require Import Base.
+Require Import FlowEquivalence.
+Require Import List.
+Import ListNotations.
+Open Scope list_scope.
+
+Require Import Omega.
+
+Require Import PeanoNat.
+
+Existing Instance event_eq_dec.
+Existing Instance latch_eq_dec.
+
+Require Import Coq.Logic.FunctionalExtensionality.
+Require Import Coq.Program.Equality.
+
+Section Desynchronization.
+
+
+  Context (even odd : Set).
+  Context `{Heven : eq_dec even} `{Hodd : eq_dec odd}.
+
+  Variable c : circuit even odd.
+  Variable init_st : state (latch even odd).
+
+
+  Inductive desync_place : event even odd -> event even odd -> Set :=
+  | Even_fall (E : even) : desync_place (Rise (Even E)) (Fall (Even E))
+  | Even_rise (E : even) : desync_place (Fall (Even E)) (Rise (Even E))
+  | Odd_fall  (O : odd) : desync_place (Rise (Odd O)) (Fall (Odd O))
+  | Odd_rise  (O : odd) : desync_place (Fall (Odd O)) (Rise (Odd O))
+  | Even_rise_odd_fall E O : In (E,O) (even_odd_neighbors c) ->
+                             desync_place (Rise (Even E)) (Fall (Odd O))
+  | Odd_fall_even_rise E O : In (E,O) (even_odd_neighbors c) ->
+                             desync_place (Fall (Odd O)) (Rise (Even E))
+  | Odd_rise_even_fall O E : In (O,E) (odd_even_neighbors c) ->
+                             desync_place (Rise (Odd O)) (Fall (Even E))
+  | Even_fall_odd_rise O E : In (O,E) (odd_even_neighbors c) ->
+                             desync_place (Fall (Even E)) (Rise (Odd O)).
+
+  Definition desynchronization : marked_graph (event even odd) :=
+    {| place := desync_place
+     ; init_marking := fun t1 t2 p => match p with
+                                      | Even_fall _ => 1
+                                      | Odd_rise  _ => 1
+                                      | Even_rise_odd_fall _ _ _ => 1
+                                      | Even_fall_odd_rise _ _ _ => 1
+                                      | _ => 0
+                                      end
+    |}.
+
+  Definition P_FD : tstate even odd :=
+    fun l => match l with
+             | Even _ => Transparent
+             | Odd _  => Opaque
+             end.
+
+Inductive is_enabled_desync : event even odd -> marking desynchronization -> Prop :=
+| Even_fall_enabled E (m : marking desynchronization) :
+  0 < m _ _ (Even_fall E) ->
+  (forall O (pf : In (O,E) (odd_even_neighbors c)),
+          0 < m _ _ (Odd_rise_even_fall O E pf)) ->
+  is_enabled_desync (Fall (Even E)) m
+| Even_rise_enabled E (m : marking desynchronization) :
+  0 < m _ _ (Even_rise E) ->
+  (forall O (pf : In (E,O) (even_odd_neighbors c)),
+          0 < m _ _ (Odd_fall_even_rise E O pf)) ->
+  is_enabled_desync (Rise (Even E)) m
+| Odd_fall_enabled O (m : marking desynchronization) :
+  0 < m _ _ (Odd_fall O) ->
+  (forall E (pf : In (E,O) (even_odd_neighbors c)),
+          0 < m _ _ (Even_rise_odd_fall E O pf)) ->
+  is_enabled_desync (Fall (Odd O)) m
+| Odd_rise_enabled O (m : marking desynchronization) :
+  0 < m _ _ (Odd_rise O) ->
+  (forall E (pf : In (O,E) (odd_even_neighbors c)),
+          0 < m _ _ (Even_fall_odd_rise O E pf)) ->
+  is_enabled_desync (Rise (Odd O)) m
+
+.
+
+
+
+Lemma desync_is_enabled_equiv : forall e m,
+    is_enabled_desync e m -> is_enabled desynchronization e m.
+Proof.
+  destruct e as [[O | E] | [O | E]];
+    intros m; inversion 1; subst;
+    intros e0 p;
+    simpl in p;
+    dependent destruction p;
+    auto.
+Qed.
+
+
+Lemma is_enabled_desync_equiv : forall e m,
+    is_enabled desynchronization e m ->
+    is_enabled_desync e m.
+Proof.
+  intros e m Henabled.
+  unfold is_enabled in *.
+  destruct e as [[O | E] | [O | E]];
+    constructor; intros; apply Henabled; eexists; try (econstructor; eauto; fail).
+Qed.
+
+
+End Desynchronization.
+
+Arguments P_FD {even odd}.
+Arguments desynchronization {even odd}.
+
+Section Counterexample.
+
+
+  Inductive d_even := A | C.
+  Inductive d_odd := B.
+  Instance d_even_eq_dec : eq_dec d_even.
+  Proof. 
+    split. intros [ | ] [ | ];
+      try (left; reflexivity); try (right; discriminate).
+  Defined.
+  Instance d_odd_eq_dec : eq_dec d_odd.
+  Proof. 
+    split. intros [ ] [ ];
+      try (left; reflexivity).
+  Defined.
+
+
+  Variable next_state_A : unit -> value.
+  Variable next_state_B : value -> value.
+  Variable next_state_C : value -> value.
+
+  Program Definition c : circuit d_even d_odd :=
+    {| even_odd_neighbors := [ (A,B) ]
+     ; odd_even_neighbors := [ (B,C) ]
+     ; next_state_e := fun e =>
+        match e with
+        | A => fun _ => next_state_A tt
+        | C => fun st => next_state_C (st (existT _ B _))
+        end
+     ; next_state_o := fun o =>
+        match o with
+        | B => fun st => next_state_B (st (existT _ A _))
+        end
+     |}.
+
+  Lemma exists_not_forall : forall A (P : A -> Prop),
+    (exists x, ~P x) ->
+    ~ forall x, P x.
+  Proof.
+    intros A P [x H] contr.
+    specialize (contr x).
+    contradiction.
+  Qed.
+
+
+Lemma c_odd_even_neighbors : forall O E,
+    In (O,E) (odd_even_neighbors c) ->
+    O = B /\ E = C.
+Proof.
+    intros O E [H | []].
+    inversion H.
+    auto.
+Qed.
+Lemma c_even_odd_neighbors : forall E O,
+    In (E,O) (even_odd_neighbors c) ->
+    E = A /\ O = B.
+Proof.
+    intros E O [H | []].
+    inversion H.
+    auto.
+Qed.
+
+
+  Variable init_st : state (latch d_even d_odd).
+
+  Definition counter_trace : trace d_even d_odd :=
+    t_empty :> Rise (Odd B) :> Fall (Odd B) 
+            :> Fall (Even C) :> Rise (Even C)
+            :> Rise (Odd B) :> Fall (Even C)
+            :> Fall (Even A) :> Rise (Even A)
+            :> Fall (Odd B)
+            :> Fall (Even A) :> Rise (Even A) :> Fall (Even A)
+            :> Rise (Odd B) :> Fall (Odd B)
+            :> Rise (Even C) :> Fall (Even C).
+
+    
+Ltac inversion_neighbors :=
+  repeat match goal with
+  | [ H : neighbor c _ _ |- _ ] =>
+    inversion H; clear H
+  | [ H : In (_, _) (odd_even_neighbors c) |- _ ] =>
+    destruct (c_odd_even_neighbors _ _ H); try discriminate; subst; clear
+  | [ H : In (_, _) (even_odd_neighbors c) |- _ ] =>
+    destruct (c_even_odd_neighbors _ _ H); try discriminate; subst; clear
+  end.
+
+    
+
+  Lemma counter_trace_well_formed : exists m, 
+    { desynchronization c }⊢ counter_trace ↓ m.
+  Proof.
+    eexists.
+    unfold counter_trace.
+  
+    repeat (try (econstructor; [ | reflexivity | ])); try (econstructor; fail);
+
+    apply desync_is_enabled_equiv; constructor; auto; intros;
+    inversion_neighbors;
+       try (repeat (unfold fire at 1; simpl; auto); fail).
+  Qed.    
+
+ Lemma counter_eval :
+    ⟨c,init_st,P_FD⟩⊢ counter_trace ↓ Even C ↦{Opaque}
+        sync_eval c init_st 2 (Even C).
+  Proof.
+    unfold counter_trace.
+
+    set (st := fun (l0 : latch d_even d_odd) =>
+             match l0 with
+             | Even A => next_state_A tt
+             | Odd B => next_state_B (next_state_A tt)
+             | Even C => next_state_C (next_state_B (next_state_A tt))
+             end).
+    apply async_opaque_fall with (st := st); [reflexivity | | reflexivity ].
+    intros l' Hl'.
+    inversion_neighbors.
+    constructor; [ reflexivity | discriminate | ].
+    apply async_opaque_fall with (st := st); [reflexivity | | reflexivity ].
+    intros l' Hl'.
+    inversion_neighbors.
+    simpl.
+    constructor; [ reflexivity | discriminate | ].
+    apply async_opaque_fall with (st := st); [reflexivity | | reflexivity ].
+    intros l' Hl'. inversion_neighbors.
+  Qed.    
+
+  (* In the Coq model, this is not technically true, since the value of A will
+     always be next_state_A (), which is determinsitic. How to refine this??
+
+     1. Let values in the formalization be abstract, and initialize them with a
+   monad with internal state that can update over time.
+
+     2. Encode environment?
+
+     3. Consider only the 6-state cycle, which is closed.
+ *)
+  Hypothesis sync_2_3_neq :
+    sync_eval c init_st 2 (Even C) <> sync_eval c init_st 3 (Even C).
+
+  Theorem desynchronization_not_flow_equivalent :
+    ~ flow_equivalence (desynchronization c) c init_st P_FD.
+  Proof.
+    unfold flow_equivalence.
+    apply exists_not_forall.
+    exists (Even C).
+    apply exists_not_forall.
+    exists counter_trace.
+    apply exists_not_forall.
+    exists (sync_eval c init_st 2 (Even C)).
+    apply exists_not_forall.
+    exists (counter_trace_well_formed).
+    apply exists_not_forall.
+    exists counter_eval.
+
+    replace (num_events (Fall (Even C)) counter_trace) with 3 by reflexivity.
+
+    apply sync_2_3_neq.
+  Qed.
+
+
+End Counterexample.
